Separate definitions for HashMap and HashSet

src/Std/Data/HashSet/Basic.lean
@@ -7,15 +7,18 @@ prelude
 import Std.Data.HashMap.Basic
 
 /-!
-# Hash set
+# Hash sets
 
-This file develops the two types `Std.Data.HashSet.Raw` and `Std.Data.HashSet`. The difference between these
-types is that the former does not bundle the well-formedness invariant and is thus safe to use in
-nested inductive types. The well-formedness predicate is available as `Std.Data.HashSet.Raw.WF` and this
-file proves that all operations preserve well-formedness.
+This file develops the type `Std.Data.HashSet` of dependent hash sets.
 
-Lemmas about the operations on `Std.Data.HashSet.Raw` and `Std.Data.HashSet` are available in the module
-`Std.Data.HashSet.Lemmas`.
+The operations `map` and `filterMap` on `Std.Data.HashSet` are defined in the module
+`Std.Data.HashSet.AdditionalOperations`.
+
+Lemmas about the operations on `Std.Data.HashSet` are available in the
+module `Std.Data.HashSet.Lemmas`.
+
+See the module `Std.Data.HashSet.Raw` for a variant of this type which is safe to use in
+nested inductive types.
 -/
 
 set_option linter.missingDocs true
@@ -26,120 +29,6 @@ universe u v
 variable {α : Type u}
 
 namespace Std
-
-namespace HashSet
-
-structure Raw (α : Type u) where
-  inner : HashMap.Raw α Unit
-
-namespace Raw
-
-@[inline] def empty (capacity := 8) : Raw α :=
-  ⟨HashMap.Raw.empty capacity⟩
-
-instance : EmptyCollection (Raw α) where
-  emptyCollection := empty
-
-@[inline] def insert [BEq α] [Hashable α] (m : Raw α) (a : α) : Raw α :=
-  ⟨m.inner.insert a ()⟩
-
-@[inline] def containsThenInsert [BEq α] [Hashable α] (m : Raw α) (a : α) : Bool × Raw α :=
-  let ⟨replaced, r⟩ := m.inner.containsThenInsert a ()
-  ⟨replaced, ⟨r⟩⟩
-
-@[inline] def contains [BEq α] [Hashable α] (m : Raw α) (a : α) : Bool :=
-  m.inner.contains a
-
-instance [BEq α] [Hashable α] : Membership α (Raw α) where
-  mem a m := a ∈ m.inner
-
-instance [BEq α] [Hashable α] {m : Raw α} {a : α} : Decidable (a ∈ m) :=
-  inferInstanceAs (Decidable (a ∈ m.inner))
-
-@[inline] def remove [BEq α] [Hashable α] (m : Raw α) (a : α) : Raw α :=
-  ⟨m.inner.remove a⟩
-
-@[inline] def size (m : Raw α) : Nat :=
-  m.inner.size
-
-@[inline] def isEmpty (m : Raw α) : Bool :=
-  m.inner.isEmpty
-
-section Unverified
-
-/-! We currently do not provide lemmas for the functions below. -/
-
-@[inline] def filter [BEq α] [Hashable α] (f : α → Bool) (m : Raw α) : Raw α :=
-  ⟨m.inner.filter fun a _ => f a⟩
-
-@[inline] def foldlM {m : Type v → Type v} [Monad m] {β : Type v} (f : β → α → m β) (init : β) (b : Raw α) : m β :=
-  b.inner.foldlM (fun b a _ => f b a) init
-
-@[inline] def foldl {β : Type v} (f : β → α → β) (init : β) (m : Raw α) : β :=
-  m.inner.foldl (fun b a _ => f b a) init
-
-@[inline] def forM {m : Type v → Type v} [Monad m] (f : α → m PUnit) (b : Raw α) : m PUnit :=
-  b.inner.forM (fun a _ => f a)
-
-@[inline] def forIn {m : Type v → Type v} [Monad m] {β : Type v} (f : α → β → m (ForInStep β)) (init : β) (b : Raw α) : m β :=
-  b.inner.forIn (fun a _ acc => f a acc) init
-
-instance {m : Type v → Type v} : ForM m (Raw α) α where
-  forM m f := m.forM f
-
-instance {m : Type v → Type v} : ForIn m (Raw α) α where
-  forIn m init f := m.forIn f init
-
-@[inline] def toList (m : Raw α) : List α :=
-  m.inner.keys
-
-@[inline] def toArray (m : Raw α) : Array α :=
-  m.inner.keysArray
-
-@[inline] def insertMany [BEq α] [Hashable α] {ρ : Type v} [ForIn Id ρ α] (m : Raw α) (l : ρ) : Raw α :=
-  ⟨m.inner.insertManyUnit l⟩
-
-@[inline] def ofList [BEq α] [Hashable α] {ρ : Type v} [ForIn Id ρ α] (l : ρ) : Raw α :=
-  ⟨HashMap.Raw.unitOfList l⟩
-
-def Internal.numBuckets (m : Raw α) : Nat :=
-  HashMap.Raw.Internal.numBuckets m.inner
-
-instance [Repr α] : Repr (Raw α) where
-  reprPrec m prec := Repr.addAppParen ("Std.HashSet.Raw.ofList " ++ reprArg m.toList) prec
-
-end Unverified
-
-structure WF [BEq α] [Hashable α] (m : Raw α) : Prop where
-  out : m.inner.WF
-
-theorem WF.empty [BEq α] [Hashable α] {c} : (empty c : Raw α).WF :=
-  ⟨HashMap.Raw.WF.empty⟩
-
-theorem WF.emptyc [BEq α] [Hashable α] : (∅ : Raw α).WF :=
-  ⟨HashMap.Raw.WF.empty⟩
-
-theorem WF.insert [BEq α] [Hashable α] {m : Raw α} {a : α} (h : m.WF) : (m.insert a).WF :=
-  ⟨HashMap.Raw.WF.insert h.out⟩
-
-theorem WF.containsThenInsert [BEq α] [Hashable α] {m : Raw α} {a : α} (h : m.WF) : (m.containsThenInsert a).2.WF :=
-  ⟨HashMap.Raw.WF.containsThenInsert h.out⟩
-
-theorem WF.remove [BEq α] [Hashable α] {m : Raw α} {a : α} (h : m.WF) : (m.remove a).WF :=
-  ⟨HashMap.Raw.WF.remove h.out⟩
-
-theorem WF.filter [BEq α] [Hashable α] {m : Raw α} {f : α → Bool} (h : m.WF) : (m.filter f).WF :=
-  ⟨HashMap.Raw.WF.filter h.out⟩
-
-theorem WF.insertMany [BEq α] [Hashable α] {ρ : Type v} [ForIn Id ρ α] {m : Raw α} {l : ρ} (h : m.WF) : (m.insertMany l).WF :=
-  ⟨HashMap.Raw.WF.insertManyUnit h.out⟩
-
-theorem WF.ofList [BEq α] [Hashable α] {ρ : Type v} [ForIn Id ρ α] {l : ρ} : (ofList l : Raw α).WF :=
-  ⟨HashMap.Raw.WF.unitOfList⟩
-
-end Raw
-
-end HashSet
 
 structure HashSet (α : Type u) [BEq α] [Hashable α] where
   inner : HashMap α Unit
