src/Std/Data/HashMap/Raw.lean
@@ -1,0 +1,203 @@
+/-
+Copyright (c) 2024 Lean FRO, LLC. All rights reserved.
+Released under Apache 2.0 license as described in the file LICENSE.
+Authors: Markus Himmel
+-/
+prelude
+import Std.Data.DHashMap.Raw
+
+set_option linter.missingDocs true
+set_option autoImplicit false
+
+/-
+# Hash maps with unbundled well-formedness invariant
+
+This file develops the type `Std.Data.HashMap.Raw` of dependent hash
+maps with unbundled well-formedness invariant.
+
+This version is safe to use in nested inductive types. The well-formedness predicate is
+available as `Std.Data.HashMap.Raw.WF` and we prove in this file that all operations preserve
+well-formedness. When in doubt, prefer `HashMap` over `DHashMap.Raw`.
+
+Lemmas about the operations on `Std.Data.HashMap.Raw` are available in the module
+`Std.Data.HashMap.RawLemmas`.
+-/
+
+universe u v w
+
+variable {α : Type u} {β : Type v}
+
+namespace Std
+
+namespace HashMap
+
+structure Raw (α : Type u) (β : Type v) where
+  inner : DHashMap.Raw α (fun _ => β)
+
+namespace Raw
+
+@[inline] def empty (capacity := 8) : Raw α β :=
+  ⟨DHashMap.Raw.empty capacity⟩
+
+instance : EmptyCollection (Raw α β) where
+  emptyCollection := empty
+
+@[inline] def insert [BEq α] [Hashable α] (m : Raw α β) (a : α) (b : β) : Raw α β :=
+  ⟨m.inner.insert a b⟩
+
+@[inline] def insertIfNew [BEq α] [Hashable α] (m : Raw α β) (a : α) (b : β) : Raw α β :=
+  ⟨m.inner.insertIfNew a b⟩
+
+@[inline] def containsThenInsert [BEq α] [Hashable α] (m : Raw α β) (a : α) (b : β) : Bool × Raw α β :=
+  let ⟨replaced, r⟩ := m.inner.containsThenInsert a b
+  ⟨replaced, ⟨r⟩⟩
+
+@[inline] def getThenInsertIfNew? [BEq α] [Hashable α] (m : Raw α β) (a : α) (b : β) : Option β × Raw α β :=
+  let ⟨previous, r⟩ := DHashMap.Raw.Const.getThenInsertIfNew? m.inner a b
+  ⟨previous, ⟨r⟩⟩
+
+@[inline] def get? [BEq α] [Hashable α] (m : Raw α β) (a : α) : Option β :=
+  DHashMap.Raw.Const.get? m.inner a
+
+@[inline] def contains [BEq α] [Hashable α] (m : Raw α β) (a : α) : Bool :=
+  m.inner.contains a
+
+instance [BEq α] [Hashable α] : Membership α (Raw α β) where
+  mem a m := a ∈ m.inner
+
+instance [BEq α] [Hashable α] {m : Raw α β} {a : α} : Decidable (a ∈ m) :=
+  inferInstanceAs (Decidable (a ∈ m.inner))
+
+@[inline] def get [BEq α] [Hashable α] (m : Raw α β) (a : α) (h : a ∈ m) : β :=
+  DHashMap.Raw.Const.get m.inner a h
+
+@[inline] def getD [BEq α] [Hashable α] (m : Raw α β) (a : α) (fallback : β) : β :=
+  DHashMap.Raw.Const.getD m.inner a fallback
+
+@[inline] def get! [BEq α] [Hashable α] [Inhabited β] (m : Raw α β) (a : α) : β :=
+  DHashMap.Raw.Const.get! m.inner a
+
+instance [BEq α] [Hashable α] : GetElem? (Raw α β) α β (fun m a => a ∈ m) where
+  getElem m a h := m.get a h
+  getElem? m a := m.get? a
+  getElem! m a := m.get! a
+
+@[inline] def remove [BEq α] [Hashable α] (m : Raw α β) (a : α) : Raw α β :=
+  ⟨m.inner.remove a⟩
+
+@[inline] def size (m : Raw α β) : Nat :=
+  m.inner.size
+
+@[inline] def isEmpty (m : Raw α β) : Bool :=
+  m.inner.isEmpty
+
+section Unverified
+
+/-! We currently do not provide lemmas for the functions below. -/
+
+@[inline] def filterMap {γ : Type w} (f : α → β → Option γ) (m : Raw α β) : Raw α γ :=
+  ⟨m.inner.filterMap f⟩
+
+@[inline] def map {γ : Type w} (f : α → β → γ) (m : Raw α β) : Raw α γ :=
+  ⟨m.inner.map f⟩
+
+@[inline] def filter (f : α → β → Bool) (m : Raw α β) : Raw α β :=
+  ⟨m.inner.filter f⟩
+
+@[inline] def foldlM {m : Type w → Type w} [Monad m] {γ : Type w} (f : γ → α → β → m γ) (init : γ) (b : Raw α β) : m γ :=
+  b.inner.foldlM f init
+
+@[inline] def foldl {γ : Type w} (f : γ → α → β → γ) (init : γ) (b : Raw α β) : γ :=
+  b.inner.foldl f init
+
+@[inline] def forM {m : Type w → Type w} [Monad m] (f : (a : α) → β → m PUnit) (b : Raw α β) : m PUnit :=
+  b.inner.forM f
+
+@[inline] def forIn {m : Type w → Type w} [Monad m] {γ : Type w} (f : (a : α) → β → γ → m (ForInStep γ)) (init : γ) (b : Raw α β) : m γ :=
+  b.inner.forIn f init
+
+instance {m : Type w → Type w} : ForM m (Raw α β) (α × β) where
+  forM m f := m.forM (fun a b => f (a, b))
+
+instance {m : Type w → Type w} : ForIn m (Raw α β) (α × β) where
+  forIn m init f := m.forIn (fun a b acc => f (a, b) acc) init
+
+@[inline] def toList (m : Raw α β) : List (α × β) :=
+  DHashMap.Raw.Const.toList m.inner
+
+@[inline] def toArray (m : Raw α β) : Array (α × β) :=
+  DHashMap.Raw.Const.toArray m.inner
+
+@[inline] def keys (m : Raw α β) : List α :=
+  m.inner.keys
+
+@[inline] def keysArray (m : Raw α β) : Array α :=
+  m.inner.keysArray
+
+@[inline] def values (m : Raw α β) : List β :=
+  m.inner.values
+
+@[inline] def insertMany [BEq α] [Hashable α] {ρ : Type w} [ForIn Id ρ (α × β)] (m : Raw α β) (l : ρ) : Raw α β :=
+  ⟨DHashMap.Raw.Const.insertMany m.inner l⟩
+
+@[inline] def insertManyUnit [BEq α] [Hashable α] {ρ : Type w} [ForIn Id ρ α] (m : Raw α Unit) (l : ρ) : Raw α Unit :=
+  ⟨DHashMap.Raw.Const.insertManyUnit m.inner l⟩
+
+@[inline] def ofList [BEq α] [Hashable α] {ρ : Type w} [ForIn Id ρ (α × β)] (l : ρ) : Raw α β :=
+  ⟨DHashMap.Raw.Const.ofList l⟩
+
+@[inline] def unitOfList [BEq α] [Hashable α] {ρ : Type w} [ForIn Id ρ α] (l : ρ) : Raw α Unit :=
+  ⟨DHashMap.Raw.Const.unitOfList l⟩
+
+def Internal.numBuckets (m : Raw α β) : Nat :=
+  DHashMap.Raw.Internal.numBuckets m.inner
+
+instance [Repr α] [Repr β] : Repr (Raw α β) where
+  reprPrec m prec := Repr.addAppParen ("Std.HashMap.Raw.ofList " ++ reprArg m.toList) prec
+
+end Unverified
+
+structure WF [BEq α] [Hashable α] (m : Raw α β) : Prop where
+  out : m.inner.WF
+
+theorem WF.empty [BEq α] [Hashable α] {c} : (empty c : Raw α β).WF :=
+  ⟨DHashMap.Raw.WF.empty⟩
+
+theorem WF.emptyc [BEq α] [Hashable α] : (∅ : Raw α β).WF :=
+  WF.empty
+
+theorem WF.insert [BEq α] [Hashable α] {m : Raw α β} {a : α} {b : β} (h : m.WF) : (m.insert a b).WF :=
+  ⟨DHashMap.Raw.WF.insert h.out⟩
+
+theorem WF.insertIfNew [BEq α] [Hashable α] {m : Raw α β} {a : α} {b : β} (h : m.WF) : (m.insertIfNew a b).WF :=
+  ⟨DHashMap.Raw.WF.insertIfNew h.out⟩
+
+theorem WF.containsThenInsert [BEq α] [Hashable α] {m : Raw α β} {a : α} {b : β} (h : m.WF) : (m.containsThenInsert a b).2.WF :=
+  ⟨DHashMap.Raw.WF.containsThenInsert h.out⟩
+
+theorem WF.getThenInsertIfNew? [BEq α] [Hashable α] {m : Raw α β} {a : α} {b : β} (h : m.WF) : (m.getThenInsertIfNew? a b).2.WF :=
+  ⟨DHashMap.Raw.WF.Const.getThenInsertIfNew? h.out⟩
+
+theorem WF.remove [BEq α] [Hashable α] {m : Raw α β} {a : α} (h : m.WF) : (m.remove a).WF :=
+  ⟨DHashMap.Raw.WF.remove h.out⟩
+
+theorem WF.filter [BEq α] [Hashable α] {m : Raw α β} {f : α → β → Bool} (h : m.WF) : (m.filter f).WF :=
+  ⟨DHashMap.Raw.WF.filter h.out⟩
+
+theorem WF.insertMany [BEq α] [Hashable α] {ρ : Type w} [ForIn Id ρ (α × β)] {m : Raw α β} {l : ρ} (h : m.WF) : (m.insertMany l).WF :=
+  ⟨DHashMap.Raw.WF.Const.insertMany h.out⟩
+
+theorem WF.insertManyUnit [BEq α] [Hashable α] {ρ : Type w} [ForIn Id ρ α] {m : Raw α Unit} {l : ρ} (h : m.WF) : (m.insertManyUnit l).WF :=
+  ⟨DHashMap.Raw.WF.Const.insertManyUnit h.out⟩
+
+theorem WF.ofList [BEq α] [Hashable α] {ρ : Type w} [ForIn Id ρ (α × β)] {l : ρ} : (ofList l).WF :=
+  ⟨DHashMap.Raw.WF.Const.ofList⟩
+
+theorem WF.unitOfList [BEq α] [Hashable α] {ρ : Type w} [ForIn Id ρ α] {l : ρ} : (unitOfList l).WF :=
+  ⟨DHashMap.Raw.WF.Const.unitOfList⟩
+
+end Raw
+
+end HashMap
+
+end Std
