src/Std/Data/HashSet/Raw.lean
@@ -1,0 +1,146 @@
+/-
+Copyright (c) 2024 Lean FRO, LLC. All rights reserved.
+Released under Apache 2.0 license as described in the file LICENSE.
+Authors: Markus Himmel
+-/
+prelude
+import Std.Data.HashMap.Raw
+
+/-
+# Hash sets with unbundled well-formedness invariant
+
+This file develops the type `Std.Data.HashSet.Raw` of dependent hash
+maps with unbundled well-formedness invariant.
+
+This version is safe to use in nested inductive types. The well-formedness predicate is
+available as `Std.Data.HashSet.Raw.WF` and we prove in this file that all operations preserve
+well-formedness. When in doubt, prefer `HashSet` over `DHashSet.Raw`.
+
+Lemmas about the operations on `Std.Data.HashSet.Raw` are available in the module
+`Std.Data.HashSet.RawLemmas`.
+-/
+
+set_option linter.missingDocs true
+set_option autoImplicit false
+
+universe u v
+
+variable {α : Type u}
+
+namespace Std
+
+namespace HashSet
+
+structure Raw (α : Type u) where
+  inner : HashMap.Raw α Unit
+
+namespace Raw
+
+@[inline] def empty (capacity := 8) : Raw α :=
+  ⟨HashMap.Raw.empty capacity⟩
+
+instance : EmptyCollection (Raw α) where
+  emptyCollection := empty
+
+@[inline] def insert [BEq α] [Hashable α] (m : Raw α) (a : α) : Raw α :=
+  ⟨m.inner.insert a ()⟩
+
+@[inline] def containsThenInsert [BEq α] [Hashable α] (m : Raw α) (a : α) : Bool × Raw α :=
+  let ⟨replaced, r⟩ := m.inner.containsThenInsert a ()
+  ⟨replaced, ⟨r⟩⟩
+
+@[inline] def contains [BEq α] [Hashable α] (m : Raw α) (a : α) : Bool :=
+  m.inner.contains a
+
+instance [BEq α] [Hashable α] : Membership α (Raw α) where
+  mem a m := a ∈ m.inner
+
+instance [BEq α] [Hashable α] {m : Raw α} {a : α} : Decidable (a ∈ m) :=
+  inferInstanceAs (Decidable (a ∈ m.inner))
+
+@[inline] def remove [BEq α] [Hashable α] (m : Raw α) (a : α) : Raw α :=
+  ⟨m.inner.remove a⟩
+
+@[inline] def size (m : Raw α) : Nat :=
+  m.inner.size
+
+@[inline] def isEmpty (m : Raw α) : Bool :=
+  m.inner.isEmpty
+
+section Unverified
+
+/-! We currently do not provide lemmas for the functions below. -/
+
+@[inline] def filter [BEq α] [Hashable α] (f : α → Bool) (m : Raw α) : Raw α :=
+  ⟨m.inner.filter fun a _ => f a⟩
+
+@[inline] def foldlM {m : Type v → Type v} [Monad m] {β : Type v} (f : β → α → m β) (init : β) (b : Raw α) : m β :=
+  b.inner.foldlM (fun b a _ => f b a) init
+
+@[inline] def foldl {β : Type v} (f : β → α → β) (init : β) (m : Raw α) : β :=
+  m.inner.foldl (fun b a _ => f b a) init
+
+@[inline] def forM {m : Type v → Type v} [Monad m] (f : α → m PUnit) (b : Raw α) : m PUnit :=
+  b.inner.forM (fun a _ => f a)
+
+@[inline] def forIn {m : Type v → Type v} [Monad m] {β : Type v} (f : α → β → m (ForInStep β)) (init : β) (b : Raw α) : m β :=
+  b.inner.forIn (fun a _ acc => f a acc) init
+
+instance {m : Type v → Type v} : ForM m (Raw α) α where
+  forM m f := m.forM f
+
+instance {m : Type v → Type v} : ForIn m (Raw α) α where
+  forIn m init f := m.forIn f init
+
+@[inline] def toList (m : Raw α) : List α :=
+  m.inner.keys
+
+@[inline] def toArray (m : Raw α) : Array α :=
+  m.inner.keysArray
+
+@[inline] def insertMany [BEq α] [Hashable α] {ρ : Type v} [ForIn Id ρ α] (m : Raw α) (l : ρ) : Raw α :=
+  ⟨m.inner.insertManyUnit l⟩
+
+@[inline] def ofList [BEq α] [Hashable α] {ρ : Type v} [ForIn Id ρ α] (l : ρ) : Raw α :=
+  ⟨HashMap.Raw.unitOfList l⟩
+
+def Internal.numBuckets (m : Raw α) : Nat :=
+  HashMap.Raw.Internal.numBuckets m.inner
+
+instance [Repr α] : Repr (Raw α) where
+  reprPrec m prec := Repr.addAppParen ("Std.HashSet.Raw.ofList " ++ reprArg m.toList) prec
+
+end Unverified
+
+structure WF [BEq α] [Hashable α] (m : Raw α) : Prop where
+  out : m.inner.WF
+
+theorem WF.empty [BEq α] [Hashable α] {c} : (empty c : Raw α).WF :=
+  ⟨HashMap.Raw.WF.empty⟩
+
+theorem WF.emptyc [BEq α] [Hashable α] : (∅ : Raw α).WF :=
+  ⟨HashMap.Raw.WF.empty⟩
+
+theorem WF.insert [BEq α] [Hashable α] {m : Raw α} {a : α} (h : m.WF) : (m.insert a).WF :=
+  ⟨HashMap.Raw.WF.insert h.out⟩
+
+theorem WF.containsThenInsert [BEq α] [Hashable α] {m : Raw α} {a : α} (h : m.WF) : (m.containsThenInsert a).2.WF :=
+  ⟨HashMap.Raw.WF.containsThenInsert h.out⟩
+
+theorem WF.remove [BEq α] [Hashable α] {m : Raw α} {a : α} (h : m.WF) : (m.remove a).WF :=
+  ⟨HashMap.Raw.WF.remove h.out⟩
+
+theorem WF.filter [BEq α] [Hashable α] {m : Raw α} {f : α → Bool} (h : m.WF) : (m.filter f).WF :=
+  ⟨HashMap.Raw.WF.filter h.out⟩
+
+theorem WF.insertMany [BEq α] [Hashable α] {ρ : Type v} [ForIn Id ρ α] {m : Raw α} {l : ρ} (h : m.WF) : (m.insertMany l).WF :=
+  ⟨HashMap.Raw.WF.insertManyUnit h.out⟩
+
+theorem WF.ofList [BEq α] [Hashable α] {ρ : Type v} [ForIn Id ρ α] {l : ρ} : (ofList l : Raw α).WF :=
+  ⟨HashMap.Raw.WF.unitOfList⟩
+
+end Raw
+
+end HashSet
+
+end Std
